vyperSmallStepScript.sml
@@ -57,7 +57,7 @@ Datatype:
   | BuiltinK builtin eval_continuation
   | TypeBuiltinK type_builtin type eval_continuation
   | CallSendK eval_continuation
-  | IntCallK (num |-> type_args) identifier ((identifier # type) list) type (stmt list) eval_continuation
+  | IntCallK (num |-> type_args) (num option # identifier) ((identifier # type) list) type (stmt list) eval_continuation
   | IntCallK1 (scope list) type_value eval_continuation
   | ExprsK (expr list) eval_continuation
   | ExprsK1 value eval_continuation
@@ -90,7 +90,7 @@ End
 val liftk1 = oneline liftk_def;
 
 Definition no_recursion_def:
-  no_recursion (fn:identifier) stk ⇔ ¬MEM fn stk
+  no_recursion (src_fn : num option # identifier) stk ⇔ ¬MEM src_fn stk
 End
 
 val () = cv_auto_trans no_recursion_def;
@@ -184,8 +184,8 @@ Definition eval_expr_cps_def:
     AK cx10 (ApplyExc (Error "TODO: ExtCall")) st k ∧
   eval_expr_cps cx10 (Call (IntCall ns fn) es) st k =
     (case do
-      check (no_recursion fn cx10.stk) "recursion";
-      ts <- lift_option (get_self_code cx10) "IntCall get_self_code";
+      check (no_recursion (ns, fn) cx10.stk) "recursion";
+      ts <- lift_option (get_module_code cx10 ns) "IntCall get_module_code";
       tup <- lift_option (lookup_function fn Internal ts) "IntCall lookup_function";
       stup <<- SND tup; args <<- FST stup; sstup <<- SND stup;
       ret <<- FST $ sstup; body <<- SND $ sstup;
@@ -193,7 +193,7 @@ Definition eval_expr_cps_def:
       return (type_env ts, args, ret, body) od st
      of (INR ex, st) => AK cx10 (ApplyExc ex) st k
       | (INL (tenv, args, ret, body), st) =>
-          eval_exprs_cps cx10 es st (IntCallK tenv fn args ret body k)) ∧
+          eval_exprs_cps cx10 es st (IntCallK tenv (ns, fn) args ret body k)) ∧
   eval_exprs_cps cx11 [] st k = AK cx11 (ApplyVals []) st k ∧
   eval_exprs_cps cx12 (e::es) st k =
     eval_expr_cps cx12 e st (ExprsK es k)
@@ -577,12 +577,12 @@ Definition apply_vals_def:
       transfer_value cx.txn.target toAddr amount;
       return $ Value NoneV
     od st) k ∧
-  apply_vals cx vs st (IntCallK tenv fn args ret body k) =
+  apply_vals cx vs st (IntCallK tenv src_fn args ret body k) =
     (case do
       env <- lift_option (bind_arguments tenv args vs) "IntCall bind_arguments";
       prev <- get_scopes;
       rtv <- lift_option (evaluate_type tenv ret) "IntCall eval ret";
-      cxf <- push_function fn env cx;
+      cxf <- push_function src_fn env cx;
       return (prev, cxf, body, rtv) od st
      of (INR ex, st) => apply_exc cx ex st k
       | (INL (prev, cxf, body, rtv), st) =>
